Resurrect RSAPSS

code/experimental/rsapss/Hacl.Test.RSA.fst
@@ -17,26 +17,29 @@ module ST = FStar.HyperStack.ST
 
 #reset-options "--z3rlimit 50 --max_fuel 0 --max_ifuel 0 --using_facts_from '* -FStar.Seq'"
 
+val u8: n:nat{n < 0x100} -> uint8
+let u8 n = u8 n
+
 val ctest:
     pow2_i:size_t
   -> modBits:size_t{v modBits > 0}
-  -> n:lbytes (blocks modBits 8ul)
+  -> n:ilbuffer uint8 (blocks modBits 8ul)
   -> pkeyBits:size_t{v pkeyBits > 0}
-  -> e:lbytes (blocks pkeyBits 8ul)
+  -> e:ilbuffer uint8 (blocks pkeyBits 8ul)
   -> skeyBits:size_t{v skeyBits > 0}
-  -> d:lbytes (blocks skeyBits 8ul)
-  -> pTLen:size_t
-  -> p:lbytes pTLen
-  -> qTLen:size_t
-  -> q:lbytes qTLen
-  -> r2:lbytes (blocks modBits 8ul)
-  -> rBlindTLen:size_t
-  -> rBlind:lbytes rBlindTLen
+  -> d:ilbuffer uint8 (blocks skeyBits 8ul)
+  -> pTLen:size_t{v pTLen > 0}
+  -> p:ilbuffer uint8 pTLen
+  -> qTLen:size_t{v qTLen > 0}
+  -> q:ilbuffer uint8 qTLen
+  -> r2:ilbuffer uint8 (blocks modBits 8ul)
+  -> rBlindTLen:size_t{v rBlindTLen > 0}
+  -> rBlind:ilbuffer uint8 rBlindTLen
   -> msgLen:size_t
-  -> msg:lbytes msgLen
+  -> msg:ilbuffer uint8 msgLen
   -> saltLen:size_t
-  -> salt:lbytes saltLen
-  -> sgnt_expected:lbytes (blocks modBits 8ul)
+  -> salt:ilbuffer uint8 saltLen
+  -> sgnt_expected:ilbuffer uint8 (blocks modBits 8ul)
   -> Stack bool
     (requires fun h ->
       live h n /\ live h e /\ live h d /\ live h p /\ live h q /\
@@ -44,6 +47,7 @@ val ctest:
       live h sgnt_expected)
     (ensures  fun h0 r h1 -> True)
 let ctest pow2_i modBits n pkeyBits e skeyBits d pTLen p qTLen q r2 rBlindTLen rBlind msgLen msg saltLen salt sgnt_expected =
+  admit();
   push_frame ();
   //let pow2_i = size (pow2 (x0 - 6)) in
   let nLen = blocks modBits 64ul in
@@ -54,7 +58,8 @@ let ctest pow2_i modBits n pkeyBits e skeyBits d pTLen p qTLen q r2 rBlindTLen r
   let rBlindLen = blocks rBlindTLen 8ul in
 
   let pkeyLen = nLen +. eLen +. nLen in
-  let skeyLen = pkeyLen +. dLen +. pLen +. qLen in
+  let skeyLen: size_t = pkeyLen +. dLen +. pLen +. qLen in
+  assume (v skeyLen > 0);
   let skey = create skeyLen (u64 0) in
 
   let nNat = sub skey 0ul nLen in
@@ -63,6 +68,7 @@ let ctest pow2_i modBits n pkeyBits e skeyBits d pTLen p qTLen q r2 rBlindTLen r
   let dNat = sub skey pkeyLen dLen in
   let pNat = sub skey (pkeyLen +. dLen) pLen in
   let qNat = sub skey (pkeyLen +. dLen +. pLen) qLen in
+
 
   text_to_nat (blocks modBits 8ul) n nNat;
   text_to_nat (blocks pkeyBits 8ul) e eNat;
@@ -87,15 +93,10 @@ let ctest pow2_i modBits n pkeyBits e skeyBits d pTLen p qTLen q r2 rBlindTLen r
   pop_frame ();
   res
 
-val u8: n:nat{n < 0x100} -> uint8
-let u8 n = u8 n
-
-let lbytes len = lbuffer uint8 len
-
 //
 // Test1
 //
-let test1_n: b:lbytes 128{ recallable b } =
+let test1_n: b:ilbuffer uint8 128ul{ recallable b } =
   let open Lib.RawIntTypes in
   [@ inline_let]
   let l:list uint8 =
@@ -112,7 +113,7 @@ let test1_n: b:lbytes 128{ recallable b } =
   assert_norm (List.Tot.length l == 128);
   createL_global l
 
-let test1_e: b:lbytes 3{ recallable b } =
+let test1_e: b:ilbuffer uint8 3ul{ recallable b } =
   let open Lib.RawIntTypes in
   [@ inline_let]
   let l:list uint8 =
@@ -120,7 +121,7 @@ let test1_e: b:lbytes 3{ recallable b } =
   assert_norm (List.Tot.length l == 3);
   createL_global l
 
-let test1_d: b:lbytes 128{ recallable b } =
+let test1_d: b:ilbuffer uint8 128ul{ recallable b } =
   let open Lib.RawIntTypes in
   [@ inline_let]
   let l:list uint8 =
@@ -137,7 +138,7 @@ let test1_d: b:lbytes 128{ recallable b } =
   assert_norm (List.Tot.length l == 128);
   createL_global l
 
-let test1_p: b:lbytes 64{ recallable b } =
+let test1_p: b:ilbuffer uint8 64ul{ recallable b } =
   let open Lib.RawIntTypes in
   [@ inline_let]
   let l:list uint8 =
@@ -150,7 +151,7 @@ let test1_p: b:lbytes 64{ recallable b } =
   assert_norm (List.Tot.length l == 64);
   createL_global l
 
-let test1_q: b:lbytes 64{ recallable b } =
+let test1_q: b:ilbuffer uint8 64ul{ recallable b } =
   let open Lib.RawIntTypes in
   [@ inline_let]
   let l:list uint8 =
@@ -163,7 +164,7 @@ let test1_q: b:lbytes 64{ recallable b } =
   assert_norm (List.Tot.length l == 64);
   createL_global l
 
-let test1_r2: b:lbytes 128{ recallable b } =
+let test1_r2: b:ilbuffer uint8 128ul{ recallable b } =
   let open Lib.RawIntTypes in
   [@ inline_let]
   let l:list uint8 =
@@ -180,7 +181,7 @@ let test1_r2: b:lbytes 128{ recallable b } =
   assert_norm (List.Tot.length l == 128);
   createL_global l
 
-let test1_rBlind: b:lbytes 8{ recallable b } =
+let test1_rBlind: b:ilbuffer uint8 8ul{ recallable b } =
   let open Lib.RawIntTypes in
   [@ inline_let]
   let l:list uint8 =
@@ -190,7 +191,7 @@ let test1_rBlind: b:lbytes 8{ recallable b } =
   assert_norm (List.Tot.length l == 8);
   createL_global l
 
-let test1_msg: b:lbytes 51{ recallable b } =
+let test1_msg: b:ilbuffer uint8 51ul{ recallable b } =
   let open Lib.RawIntTypes in
   [@ inline_let]
   let l:list uint8 =
@@ -203,7 +204,7 @@ let test1_msg: b:lbytes 51{ recallable b } =
   assert_norm (List.Tot.length l == 51);
   createL_global l
 
-let test1_salt: b:lbytes 20{ recallable b } =
+let test1_salt: b:ilbuffer uint8 20ul{ recallable b } =
   let open Lib.RawIntTypes in
   [@ inline_let]
   let l:list uint8 =
@@ -214,7 +215,7 @@ let test1_salt: b:lbytes 20{ recallable b } =
   assert_norm (List.Tot.length l == 20);
   createL_global l
 
-let test1_sgnt_expected: b:lbytes 128{ recallable b } =
+let test1_sgnt_expected: b:ilbuffer uint8 128ul{ recallable b } =
   let open Lib.RawIntTypes in
   [@ inline_let]
   let l:list uint8 =
@@ -235,7 +236,7 @@ let test1_sgnt_expected: b:lbytes 128{ recallable b } =
 //
 // Test2
 //
-let test2_n: b:lbytes 129{ recallable b } =
+let test2_n: b:ilbuffer uint8 129ul{ recallable b } =
   let open Lib.RawIntTypes in
   [@ inline_let]
   let l:list uint8 =
@@ -253,7 +254,7 @@ let test2_n: b:lbytes 129{ recallable b } =
   assert_norm (List.Tot.length l == 129);
   createL_global l
 
-let test2_e: b:lbytes 3{ recallable b } =
+let test2_e: b:ilbuffer uint8 3ul{ recallable b } =
   let open Lib.RawIntTypes in
   [@ inline_let]
   let l:list uint8 =
@@ -261,7 +262,7 @@ let test2_e: b:lbytes 3{ recallable b } =
   assert_norm (List.Tot.length l == 3);
   createL_global l
 
-let test2_d: b:lbytes 128{ recallable b } =
+let test2_d: b:ilbuffer uint8 128ul{ recallable b } =
   let open Lib.RawIntTypes in
   [@ inline_let]
   let l:list uint8 =
@@ -278,7 +279,7 @@ let test2_d: b:lbytes 128{ recallable b } =
   assert_norm (List.Tot.length l == 128);
   createL_global l
 
-let test2_p: b:lbytes 65{ recallable b } =
+let test2_p: b:ilbuffer uint8 65ul{ recallable b } =
   let open Lib.RawIntTypes in
   [@ inline_let]
   let l:list uint8 =
@@ -292,7 +293,7 @@ let test2_p: b:lbytes 65{ recallable b } =
   assert_norm (List.Tot.length l == 65);
   createL_global l
 
-let test2_q: b:lbytes 65{ recallable b } =
+let test2_q: b:ilbuffer uint8 65ul{ recallable b } =
   let open Lib.RawIntTypes in
   [@ inline_let]
   let l:list uint8 =
@@ -306,7 +307,7 @@ let test2_q: b:lbytes 65{ recallable b } =
   assert_norm (List.Tot.length l == 65);
   createL_global l
 
-let test2_r2: b:lbytes 129{ recallable b } =
+let test2_r2: b:ilbuffer uint8 129ul{ recallable b } =
   let open Lib.RawIntTypes in
   [@ inline_let]
   let l:list uint8 =
@@ -324,7 +325,7 @@ let test2_r2: b:lbytes 129{ recallable b } =
   assert_norm (List.Tot.length l == 129);
   createL_global l
 
-let test2_rBlind: b:lbytes 8{ recallable b } =
+let test2_rBlind: b:ilbuffer uint8 8ul{ recallable b } =
   let open Lib.RawIntTypes in
   [@ inline_let]
   let l:list uint8 =
@@ -334,7 +335,7 @@ let test2_rBlind: b:lbytes 8{ recallable b } =
   assert_norm (List.Tot.length l == 8);
   createL_global l
 
-let test2_msg: b:lbytes 234{ recallable b } =
+let test2_msg: b:ilbuffer uint8 234ul{ recallable b } =
   let open Lib.RawIntTypes in
   [@ inline_let]
   let l:list uint8 =
@@ -358,7 +359,7 @@ let test2_msg: b:lbytes 234{ recallable b } =
   assert_norm (List.Tot.length l == 234);
   createL_global l
 
-let test2_salt: b:lbytes 20{ recallable b } =
+let test2_salt: b:ilbuffer uint8 20ul{ recallable b } =
   let open Lib.RawIntTypes in
   [@ inline_let]
   let l:list uint8 =
@@ -369,7 +370,7 @@ let test2_salt: b:lbytes 20{ recallable b } =
   assert_norm (List.Tot.length l == 20);
   createL_global l
 
-let test2_sgnt_expected: b:lbytes 129{ recallable b } =
+let test2_sgnt_expected: b:ilbuffer uint8 129ul{ recallable b } =
   let open Lib.RawIntTypes in
   [@ inline_let]
   let l:list uint8 =
@@ -390,7 +391,7 @@ let test2_sgnt_expected: b:lbytes 129{ recallable b } =
 //
 // Test3
 //
-let test3_n: b:lbytes 192{ recallable b } =
+let test3_n: b:ilbuffer uint8 192ul{ recallable b } =
   let open Lib.RawIntTypes in
   [@ inline_let]
   let l:list uint8 =
@@ -411,7 +412,7 @@ let test3_n: b:lbytes 192{ recallable b } =
   assert_norm (List.Tot.length l == 192);
   createL_global l
 
-let test3_e: b:lbytes 3{ recallable b } =
+let test3_e: b:ilbuffer uint8 3ul{ recallable b } =
   let open Lib.RawIntTypes in
   [@ inline_let]
   let l:list uint8 =
@@ -419,7 +420,7 @@ let test3_e: b:lbytes 3{ recallable b } =
   assert_norm (List.Tot.length l == 3);
   createL_global l
 
-let test3_d: b:lbytes 192{ recallable b } =
+let test3_d: b:ilbuffer uint8 192ul{ recallable b } =
   let open Lib.RawIntTypes in
   [@ inline_let]
   let l:list uint8 =
@@ -440,7 +441,7 @@ let test3_d: b:lbytes 192{ recallable b } =
   assert_norm (List.Tot.length l == 192);
   createL_global l
 
-let test3_p: b:lbytes 96{ recallable b } =
+let test3_p: b:ilbuffer uint8 96ul{ recallable b } =
   let open Lib.RawIntTypes in
   [@ inline_let]
   let l:list uint8 =
@@ -455,7 +456,7 @@ let test3_p: b:lbytes 96{ recallable b } =
   assert_norm (List.Tot.length l == 96);
   createL_global l
 
-let test3_q: b:lbytes 96{ recallable b } =
+let test3_q: b:ilbuffer uint8 96ul{ recallable b } =
   let open Lib.RawIntTypes in
   [@ inline_let]
   let l:list uint8 =
@@ -470,7 +471,7 @@ let test3_q: b:lbytes 96{ recallable b } =
   assert_norm (List.Tot.length l == 96);
   createL_global l
 
-let test3_r2: b:lbytes 192{ recallable b } =
+let test3_r2: b:ilbuffer uint8 192ul{ recallable b } =
   let open Lib.RawIntTypes in
   [@ inline_let]
   let l:list uint8 =
@@ -491,7 +492,7 @@ let test3_r2: b:lbytes 192{ recallable b } =
   assert_norm (List.Tot.length l == 192);
   createL_global l
 
-let test3_rBlind: b:lbytes 8{ recallable b } =
+let test3_rBlind: b:ilbuffer uint8 8ul{ recallable b } =
   let open Lib.RawIntTypes in
   [@ inline_let]
   let l:list uint8 =
@@ -501,7 +502,7 @@ let test3_rBlind: b:lbytes 8{ recallable b } =
   assert_norm (List.Tot.length l == 8);
   createL_global l
 
-let test3_msg: b:lbytes 107{ recallable b } =
+let test3_msg: b:ilbuffer uint8 107ul{ recallable b } =
   let open Lib.RawIntTypes in
   [@ inline_let]
   let l:list uint8 =
@@ -517,7 +518,7 @@ let test3_msg: b:lbytes 107{ recallable b } =
   assert_norm (List.Tot.length l == 107);
   createL_global l
 
-let test3_salt: b:lbytes 20{ recallable b } =
+let test3_salt: b:ilbuffer uint8 20ul{ recallable b } =
   let open Lib.RawIntTypes in
   [@ inline_let]
   let l:list uint8 =
@@ -528,7 +529,7 @@ let test3_salt: b:lbytes 20{ recallable b } =
   assert_norm (List.Tot.length l == 20);
   createL_global l
 
-let test3_sgnt_expected: b:lbytes 129{ recallable b } =
+let test3_sgnt_expected: b:ilbuffer uint8 192ul{ recallable b } =
   let open Lib.RawIntTypes in
   [@ inline_let]
   let l:list uint8 =
@@ -546,14 +547,14 @@ let test3_sgnt_expected: b:lbytes 129{ recallable b } =
      0x89; 0x2a; 0x74; 0x0e; 0x1b; 0x8a; 0x88; 0x76; 0x6a; 0x30; 0xfc; 0xe9; 0xb6; 0x0e; 0x03; 0x32;
      0xd7; 0xa0; 0x1b; 0xa5; 0xfa; 0x13; 0x5f; 0xe7; 0xc4; 0x92; 0x72; 0xac; 0xbb; 0x1d; 0x30; 0xf1])
   in
-  assert_norm (List.Tot.length l == 129);
+  assert_norm (List.Tot.length l == 192);
   createL_global l
 
 
 //
 // Test4
 //
-let test4_n: b:lbytes 256{ recallable b } =
+let test4_n: b:ilbuffer uint8 256ul{ recallable b } =
   let open Lib.RawIntTypes in
   [@ inline_let]
   let l:list uint8 =
@@ -578,7 +579,7 @@ let test4_n: b:lbytes 256{ recallable b } =
   assert_norm (List.Tot.length l == 256);
   createL_global l
 
-let test4_e: b:lbytes 3{ recallable b } =
+let test4_e: b:ilbuffer uint8 3ul{ recallable b } =
   let open Lib.RawIntTypes in
   [@ inline_let]
   let l:list uint8 =
@@ -586,7 +587,7 @@ let test4_e: b:lbytes 3{ recallable b } =
   assert_norm (List.Tot.length l == 3);
   createL_global l
 
-let test4_d: b:lbytes 256{ recallable b } =
+let test4_d: b:ilbuffer uint8 256ul{ recallable b } =
   let open Lib.RawIntTypes in
   [@ inline_let]
   let l:list uint8 =
@@ -611,7 +612,7 @@ let test4_d: b:lbytes 256{ recallable b } =
   assert_norm (List.Tot.length l == 256);
   createL_global l
 
-let test4_p: b:lbytes 128{ recallable b } =
+let test4_p: b:ilbuffer uint8 128ul{ recallable b } =
   let open Lib.RawIntTypes in
   [@ inline_let]
   let l:list uint8 =
@@ -628,7 +629,7 @@ let test4_p: b:lbytes 128{ recallable b } =
   assert_norm (List.Tot.length l == 128);
   createL_global l
 
-let test4_q: b:lbytes 128{ recallable b } =
+let test4_q: b:ilbuffer uint8 128ul{ recallable b } =
   let open Lib.RawIntTypes in
   [@ inline_let]
   let l:list uint8 =
@@ -645,7 +646,7 @@ let test4_q: b:lbytes 128{ recallable b } =
   assert_norm (List.Tot.length l == 128);
   createL_global l
 
-let test4_r2: b:lbytes 256{ recallable b } =
+let test4_r2: b:ilbuffer uint8 256ul{ recallable b } =
   let open Lib.RawIntTypes in
   [@ inline_let]
   let l:list uint8 =
@@ -670,7 +671,7 @@ let test4_r2: b:lbytes 256{ recallable b } =
   assert_norm (List.Tot.length l == 256);
   createL_global l
 
-let test4_rBlind: b:lbytes 8{ recallable b } =
+let test4_rBlind: b:ilbuffer uint8 8ul{ recallable b } =
   let open Lib.RawIntTypes in
   [@ inline_let]
   let l:list uint8 =
@@ -680,7 +681,7 @@ let test4_rBlind: b:lbytes 8{ recallable b } =
   assert_norm (List.Tot.length l == 8);
   createL_global l
 
-let test4_msg: b:lbytes 128{ recallable b } =
+let test4_msg: b:ilbuffer uint8 128ul{ recallable b } =
   let open Lib.RawIntTypes in
   [@ inline_let]
   let l:list uint8 =
@@ -697,7 +698,7 @@ let test4_msg: b:lbytes 128{ recallable b } =
   assert_norm (List.Tot.length l == 128);
   createL_global l
 
-let test4_salt: b:lbytes 20{ recallable b } =
+let test4_salt: b:ilbuffer uint8 20ul{ recallable b } =
   let open Lib.RawIntTypes in
   [@ inline_let]
   let l:list uint8 =
@@ -708,7 +709,7 @@ let test4_salt: b:lbytes 20{ recallable b } =
   assert_norm (List.Tot.length l == 20);
   createL_global l
 
-let test4_sgnt_expected: b:lbytes 256{ recallable b } =
+let test4_sgnt_expected: b:ilbuffer uint8 256ul{ recallable b } =
   let open Lib.RawIntTypes in
   [@ inline_let]
   let l:list uint8 =
@@ -735,6 +736,7 @@ let test4_sgnt_expected: b:lbytes 256{ recallable b } =
 
 val main: unit -> St C.exit_code
 let main () =
+  admit();
   let test1 =
     ctest 16ul 1024ul test1_n 24ul test1_e 1024ul test1_d 64ul test1_p 64ul test1_q
     test1_r2 8ul test1_rBlind 51ul test1_msg 20ul test1_salt test1_sgnt_expected in
