code/experimental/rsapss/Hacl.Impl.Exponentiation.fst
@@ -15,7 +15,7 @@ open Hacl.Impl.Multiplication
 
 module ST = FStar.HyperStack.ST
 
-#reset-options "--z3rlimit 50 --max_fuel 0 --max_ifuel 0 --using_facts_from '* -FStar.Seq'"
+#reset-options "--z3rlimit 100 --max_fuel 0 --max_ifuel 0 --using_facts_from '* -FStar.Seq'"
 
 val mul_mod_mont:
     nLen:size_t
@@ -31,8 +31,8 @@ val mul_mod_mont:
     (requires fun h ->
       live h aM /\ live h bM /\ live h resM /\ live h n /\ live h st_kara /\
       disjoint st_kara aM /\ disjoint st_kara bM /\ disjoint st_kara n /\ disjoint resM st_kara)
-    (ensures  fun h0 _ h1 -> modifies (loc_union (loc_buffer resM) (loc_buffer st_kara)) h0 h1)
-[@"c_inline"]    
+    (ensures  fun h0 _ h1 -> modifies (loc_union (loc resM) (loc st_kara)) h0 h1)
+[@"c_inline"]
 let mul_mod_mont nLen rLen pow2_i n nInv_u64 st_kara aM bM resM =
   let cLen = nLen +. nLen in
   let stLen = cLen +. 4ul *. pow2_i in
@@ -56,14 +56,14 @@ val mod_exp_:
     (requires fun h ->
       live h n /\ live h b /\ live h st_kara /\ live h st_exp /\
       disjoint st_exp st_kara /\ disjoint st_kara n /\ disjoint st_kara st_exp)
-    (ensures  fun h0 _ h1 -> modifies (loc_union (loc_buffer st_exp) (loc_buffer st_kara)) h0 h1)
+    (ensures  fun h0 _ h1 -> modifies (loc_union (loc st_exp) (loc st_kara)) h0 h1)
 [@"c_inline"]
 let mod_exp_ nLen rLen pow2_i n nInv_u64 st_kara st_exp bBits bLen b =
   let aM = sub st_exp 0ul nLen in
   let accM = sub st_exp nLen nLen in
 
   let h0 = ST.get () in
-  let inv h1 i = modifies (loc_union (loc_buffer st_exp) (loc_buffer st_kara)) h0 h1 in
+  let inv h1 i = modifies (loc_union (loc st_exp) (loc st_kara)) h0 h1 in
   Lib.Loops.for 0ul bBits inv
   (fun i ->
     (if (bn_is_bit_set bLen b i) then
@@ -86,9 +86,9 @@ val mod_exp:
   -> res:lbignum nLen
   -> Stack unit
     (requires fun h -> live h n /\ live h a /\ live h b /\ live h res /\ live h r2)
-    (ensures  fun h0 _ h1 -> modifies (loc_buffer res) h0 h1)
+    (ensures  fun h0 _ h1 -> modifies (loc res) h0 h1)
 [@"c_inline"]
-let mod_exp pow2_i modBits nLen n r2 a bBits b res = admit();
+let mod_exp pow2_i modBits nLen n r2 a bBits b res =
   push_frame ();
   let rLen = nLen +. 1ul in
   let exp_r = 64ul *. rLen in
@@ -98,8 +98,9 @@ let mod_exp pow2_i modBits nLen n r2 a bBits b res = admit();
 
   let karaLen = nLen +! nLen +! 4ul *! pow2_i in
   let stLen = nLen +! nLen +! nLen +! karaLen in
-  assume (0 < v stLen);
   let st = create stLen (u64 0) in
+
+  admit();
 
   let acc  = sub st 0ul nLen in
   let aM   = sub st nLen nLen in
@@ -107,7 +108,8 @@ let mod_exp pow2_i modBits nLen n r2 a bBits b res = admit();
 
   let st_exp  = sub st nLen (nLen +. nLen) in
   let st_kara = sub st (nLen +. nLen +. nLen) karaLen in
-  let tmp     = sub #_ #(v stLen) #(v nLen + v rLen) st (nLen +. nLen +. nLen) (nLen +. rLen) in
+  //let tmp     = sub #_ #(v stLen) #(v nLen + v rLen) st (nLen +. nLen +. nLen) (nLen +. rLen) in
+  let tmp     = sub st (nLen +. nLen +. nLen) (nLen +. rLen) in
 
   acc.(0ul) <- u64 1;
   let n0 = n.(0ul) in
